src/program_proof/wal/txns_ctx.v
@@ -1,0 +1,153 @@
+From Perennial.algebra Require Import append_list.
+From Perennial.Helpers Require Import Integers List Map.
+From Perennial.program_proof.wal Require Import abstraction.
+
+From Perennial.program_proof Require Import proof_prelude.
+
+(*
+txns: list (u64 * list update.t)
+txn_id is referenced by pos, log < pos contains updates through and including upds
+[txn_id: (pos, upds)]
+*)
+
+Class txns_ctxG Σ := { txns_ctx_alist :> alistG Σ (u64 * list update.t) }.
+Definition txns_ctxΣ : gFunctors := #[alistΣ (u64 * list update.t)].
+
+Instance subG_txns_ctx Σ : subG txns_ctxΣ Σ → txns_ctxG Σ.
+Proof. solve_inG. Qed.
+
+Section goose.
+Context `{!heapG Σ} `{!txns_ctxG Σ}.
+Implicit Types (γ:gname).
+
+Definition txn_val γ txn_id (txn: u64 * list update.t): iProp Σ :=
+  list_el γ txn_id txn.
+
+Definition txn_pos γ txn_id (pos: u64) : iProp Σ :=
+  ∃ upds, txn_val γ txn_id (pos, upds).
+
+Definition txns_ctx γ txns : iProp Σ := list_ctx γ 1 txns.
+
+Theorem alloc_txns_ctx E txns :
+  ⊢ |={E}=> ∃ γtxns, txns_ctx γtxns txns.
+Proof.
+  iMod (alist_alloc txns) as (γtxns) "Hctx".
+  iExists γtxns.
+  rewrite /txns_ctx //=.
+Qed.
+
+Theorem txn_val_to_pos γ txn_id pos upds :
+  txn_val γ txn_id (pos, upds) -∗ txn_pos γ txn_id pos.
+Proof.
+  rewrite /txn_pos.
+  iIntros "Hval".
+  iExists _; iFrame.
+Qed.
+
+Lemma txns_ctx_app {γ} txns' txns : txns_ctx γ txns ==∗ txns_ctx γ (txns ++ txns').
+Proof.
+  rewrite /txns_ctx.
+  iIntros "Hctx".
+  by iMod (alist_app _ txns' with "Hctx") as "[$ _]".
+Qed.
+
+Global Instance txn_pos_timeless γ txn_id pos :
+  Timeless (txn_pos γ txn_id pos) := _.
+
+Global Instance txn_pos_persistent γ txn_id pos :
+  Persistent (txn_pos γ txn_id pos) := _.
+
+Definition txns_are γ (start: nat) (txns_sub: list (u64*list update.t)) : iProp Σ :=
+  list_subseq γ start txns_sub.
+
+Global Instance txns_are_Persistent γ start txns_sub : Persistent (txns_are γ start txns_sub).
+Proof. apply _. Qed.
+
+Theorem txns_are_sound γ txns start txns_sub :
+  txns_ctx γ txns -∗
+  txns_are γ start txns_sub -∗
+  ⌜subslice start (start + length txns_sub)%nat txns = txns_sub⌝.
+Proof.
+  iIntros "Hctx Htxns_are".
+  iDestruct (alist_subseq_lookup with "Hctx Htxns_are") as "$".
+Qed.
+
+Lemma txns_are_nil γ start : ⊢ txns_are γ start [].
+Proof.
+  iApply list_subseq_nil.
+Qed.
+
+(** * some facts about txn_ctx *)
+Theorem txn_map_to_is_txn txns (txn_id: nat) (pos: u64) upds :
+  list_to_imap txns !! txn_id = Some (pos, upds) ->
+  is_txn txns txn_id pos.
+Proof.
+  rewrite /is_txn.
+  rewrite lookup_list_to_imap.
+  by intros ->.
+Qed.
+
+Theorem alloc_txn_pos pos upds γ txns E :
+  txns_ctx γ txns ={E}=∗
+  txns_ctx γ (txns ++ [(pos, upds)]) ∗ txn_val γ (length txns) (pos, upds).
+Proof.
+  iIntros "Hctx".
+  iMod (alist_app1 (pos,upds) with "Hctx") as "[Hctx Hval]".
+  by iFrame.
+Qed.
+
+Theorem txns_ctx_complete γ txns txn_id txn :
+  txns !! txn_id = Some txn ->
+  txns_ctx γ txns -∗ txn_val γ txn_id txn.
+Proof.
+  iIntros (Hlookup) "Hctx".
+  iDestruct (alist_lookup_el with "Hctx") as "Hel"; eauto.
+Qed.
+
+Theorem txns_ctx_complete' γ txns txn_id txn :
+  txns !! txn_id = Some txn ->
+  ▷ txns_ctx γ txns -∗ ▷ txn_val γ txn_id txn ∗ ▷ txns_ctx γ txns.
+Proof.
+  iIntros (Hlookup) "Hctx".
+  iDestruct (txns_ctx_complete with "Hctx") as "#Hel"; eauto.
+Qed.
+
+Theorem txns_ctx_txn_pos γ txns txn_id pos :
+  is_txn txns txn_id pos ->
+  txns_ctx γ txns -∗ txn_pos γ txn_id pos.
+Proof.
+  intros [txn [Hlookup ->]]%fmap_Some_1.
+  rewrite txns_ctx_complete; eauto.
+  iIntros "Htxn_val".
+  destruct txn as [pos upds].
+  iExists _; iFrame.
+Qed.
+
+Theorem txn_val_valid_general γ txns txn_id txn :
+  txns_ctx γ txns -∗
+  txn_val γ txn_id txn -∗
+  ⌜txns !! txn_id = Some txn⌝.
+Proof.
+  iIntros "Hctx Htxn".
+  iDestruct (alist_lookup with "Hctx Htxn") as %Hlookup.
+  eauto.
+Qed.
+
+Theorem txn_pos_valid_general γ txns txn_id pos :
+  txns_ctx γ txns -∗
+  txn_pos γ txn_id pos -∗
+  ⌜is_txn txns txn_id pos⌝.
+Proof.
+  iIntros "Hctx Htxn".
+  iDestruct "Htxn" as (upds) "Hval".
+  iDestruct (alist_lookup with "Hctx Hval") as %Hlookup.
+  iPureIntro.
+  rewrite /is_txn Hlookup //.
+Qed.
+
+Global Instance txns_ctx_disc γ x: Discretizable (txns_ctx γ x).
+Proof.
+  rewrite /txns_ctx/list_ctx. apply _.
+Qed.
+
+End goose.
